Finished all the required changes in proofs to make it compilable

Encryptionschulze.v
@@ -13,7 +13,8 @@ Require Import ValidityExist.
 Require Import Coq.Logic.FinFun.
 Require Import Coq.Program.Basics.
 Require Import Coq.Logic.FunctionalExtensionality.
-Require Import Psatz.  
+Require Import Psatz.
+Require Import Schulze.
 Require Export CryptoAxioms.
 Require Export Cand.
 Require Export Keys.
@@ -47,6 +48,7 @@ Module Encschulze (Import C : Cand) (Import K : Keys) (Import Crp : CryptoAxioms
       intros c d. apply  all_pairsin;
                     apply cand_fin.
     Qed.
+
 
     Lemma non_empty_l_pair : forall (l : list cand), l <> [] -> all_pairs l <> [].
     Proof.
@@ -147,7 +149,7 @@ Module Encschulze (Import C : Cand) (Import K : Keys) (Import Crp : CryptoAxioms
        intros b. pose proof (decidable_valid cand b dec_cand).
        pose proof (finiteness b (all_pairs cand_all) every_cand_t) as Ht.
        destruct Ht. pose proof (X s).
-       unfold finite in X0. apply X0. exists cand_all. auto.
+       unfold finite in X0. apply X0. exists cand_all. apply cand_fin.
        right.  unfold valid, not; intros. destruct H as [f Hf].
        destruct e as [c [d [He1 [He2 He3]]]]. pose proof (Hf c d).
        destruct H. destruct H0.
@@ -189,6 +191,8 @@ Module Encschulze (Import C : Cand) (Import K : Keys) (Import Crp : CryptoAxioms
                            cand_all (fun d => v d c) (fun d => w d c) cpi (zkppermvw c).
 
 
+    (* Bring a instance *)
+    Module M := Schulze.Schulze C.
     
     (* Inductive type to capture states during the counting *)
     Inductive EState : Type :=
@@ -197,7 +201,7 @@ Module Encschulze (Import C : Cand) (Import K : Keys) (Import Crp : CryptoAxioms
     | edecrypt : (cand -> cand -> plaintext) -> EState
     | ewinners : (cand -> bool) -> EState.
   
-
+   
     (* Inductive type for counting. Indexed over a given Group, and list of ballots 
        to be counted *) 
     Inductive ECount (grp : Group) (bs : list eballot) : EState -> Type :=
@@ -247,7 +251,7 @@ Module Encschulze (Import C : Cand) (Import K : Keys) (Import Crp : CryptoAxioms
         (forall c d, verify_zero_knowledge_decryption_proof
                   grp (decm c d) (encm c d) (zkp c d) = true) ->
         ECount grp bs (edecrypt decm)
-    | ecfin dm w (d : (forall c, (wins_type dm c) + (loses_type dm c))) :
+    | ecfin dm w (d : (forall c, (M.wins_type dm c) + (M.loses_type dm c))) :
         ECount grp bs (edecrypt dm) ->
         (forall c, w c = true <-> (exists x, d c = inl x)) ->
         (forall c, w c = false <-> (exists x, d c = inr x)) ->
@@ -256,22 +260,22 @@ Module Encschulze (Import C : Cand) (Import K : Keys) (Import Crp : CryptoAxioms
 
     (* Bootstrapping the counting process *)
     Lemma ecount_all_ballot :
-      forall (bs : list eballot), existsT encm, ECount grp bs (epartial (bs, []) encm).
+      forall (bs : list eballot), existsT encm, ECount Crp.grp bs (epartial (bs, []) encm).
     Proof.
       intros.
-      remember (fun c d : cand => encrypt_message grp 0) as encm. exists encm.
-      pose proof (ecax grp bs bs encm
+      remember (fun c d : cand => encrypt_message Crp.grp 0) as encm. exists encm.
+      pose proof (ecax Crp.grp bs bs encm
                        (fun c d => 0)
                        (fun c d => construct_zero_knowledge_decryption_proof
-                                  grp privatekey (encm c d))
+                                  Crp.grp privatekey (encm c d))
                        eq_refl (fun c d => eq_refl)).
       assert (forall c d : cand,
                  verify_zero_knowledge_decryption_proof
-                   grp ((fun _ _ : cand => 0) c d)
+                   Crp.grp ((fun _ _ : cand => 0) c d)
                    (encm c d)
                    ((fun _ _ : cand =>
-                       construct_zero_knowledge_decryption_proof grp privatekey (encm c d)) c d) =
-                 true). 
+                       construct_zero_knowledge_decryption_proof
+                         Crp.grp privatekey (encm c d)) c d) = true). 
       intros.  apply verify_honest_decryption_zkp. 
       symmetry.  rewrite Heqencm. apply decryption_deterministic.
       pose proof (X H). auto.
@@ -313,7 +317,8 @@ Module Encschulze (Import C : Cand) (Import K : Keys) (Import Crp : CryptoAxioms
        valid or not. If valid then add it to encrypted marging otherwise add it invalid  
        ballot list *)
     Lemma ppartial_count_all_counted bs : forall ts inbs m,
-        ECount grp bs (epartial (ts, inbs) m) -> existsT i nm, (ECount grp bs (epartial ([], i) nm)).
+        ECount Crp.grp bs (epartial (ts, inbs) m) ->
+        existsT i nm, (ECount Crp.grp bs (epartial ([], i) nm)).
     Proof.    
       induction ts as [|u ts IHs].
       intros inbs m He.
@@ -322,24 +327,24 @@ Module Encschulze (Import C : Cand) (Import K : Keys) (Import Crp : CryptoAxioms
       (* The idea is u valid or not valid which can be shown via u -> (* row permutation *) -> v
         -> (* colume permutation *) -> w -> (* decryption *) -> b *)
       (* generate permutation pi to permute ballot*) 
-      remember (generatePermutation grp (List.length cand_all) cand_all) as pi.
+      remember (generatePermutation Crp.grp (List.length cand_all) cand_all) as pi.
       (* generate randomness S *)
-      remember (generateS grp (List.length cand_all)) as s.
+      remember (generateS Crp.grp (List.length cand_all)) as s.
       (* commit to this permutation  using randomness s*)
-      remember (generatePermutationCommitment grp (List.length cand_all) cand_all pi s) as cpi.
+      remember (generatePermutationCommitment Crp.grp (List.length cand_all) cand_all pi s) as cpi.
       (* generate zero knowledge proof of commitment *)
-      remember (zkpPermutationCommitment grp (List.length cand_all)
+      remember (zkpPermutationCommitment Crp.grp (List.length cand_all)
                                          cand_all pi cpi s) as zkpcpi.
       (* At this point I can assert that 
          verify_permutation_commitment grp (List.length cand_all) cpi zkpcpi = true 
          using the Axiom permutation_commitment_axiom *)
-      assert (verify_permutation_commitment grp (List.length cand_all) cpi zkpcpi = true).
+      assert (verify_permutation_commitment Crp.grp (List.length cand_all) cpi zkpcpi = true).
       pose proof (permutation_commitment_axiom
                     pi cpi s zkpcpi Heqcpi Heqzkpcpi). auto.
       
       (* Convert u -> rowpermute pi -> v *)
       (* Generate randomness to use in shuffle *)
-      remember (map (fun _ => generateR grp (List.length cand_all)) cand_all) as rrowlistvalues.
+      remember (map (fun _ => generateR Crp.grp (List.length cand_all)) cand_all) as rrowlistvalues.
       (* I have generated the randomness for each row and use them in shuffling. 
          It would be good idea to convert rlistvalues to rfunvalues by 
          using search_list function *)
@@ -350,12 +355,12 @@ Module Encschulze (Import C : Cand) (Import K : Keys) (Import Crp : CryptoAxioms
 
       (* get the ballot v by shuffling each row by pi and randomness R *)
       remember (fun c =>
-                  shuffle grp (List.length cand_all)
+                  shuffle Crp.grp (List.length cand_all)
                           cand_all dec_cand (u c) pi (rrowfunvalues c)) as v.
       (* construct zero knowledge proof of shuffle that v is row shuffle of u by pi
          using the same randomness R which used in shuffle *)
       remember (fun c =>
-                  shuffle_zkp grp (List.length cand_all)
+                  shuffle_zkp Crp.grp (List.length cand_all)
                               cand_all (u c) (v c) pi cpi s (rrowfunvalues c)) as zkppermuv.
       
            
@@ -363,18 +368,18 @@ Module Encschulze (Import C : Cand) (Import K : Keys) (Import Crp : CryptoAxioms
          The property here is construct matrix from u and v and comp
          This is bit tricky so I am leaving it for the moment because we need to 
          massage the axioms *)
-      assert (Ht1 : forall c, verify_row_permutation_ballot grp u v cpi zkppermuv c = true). 
+      assert (Ht1 : forall c, verify_row_permutation_ballot Crp.grp u v cpi zkppermuv c = true). 
       intros; unfold verify_row_permutation_ballot.
       pose proof (verify_shuffle_axiom pi cpi s (u c) (v c) (rrowfunvalues c) (zkppermuv c)
                                        Heqcpi).
-      assert (Hvr : v c = shuffle grp (List.length cand_all)
+      assert (Hvr : v c = shuffle Crp.grp (List.length cand_all)
                                   cand_all dec_cand (u c) pi (rrowfunvalues c)).
       rewrite Heqv; try auto.
       specialize (H1 Hvr). clear Hvr. rewrite Heqzkppermuv in H1.
       specialize (H1 eq_refl). rewrite Heqzkppermuv; try auto. 
 
       (* generate again the randomness R to make cryptography great again *)
-      remember (map (fun _ => generateR grp (List.length cand_all)) cand_all) as rcollistvalues.
+      remember (map (fun _ => generateR Crp.grp (List.length cand_all)) cand_all) as rcollistvalues.
       (* I have generated the randomness for each column and use them in shuffling. 
          It would be good idea to convert rcollistvalues to rcolfunvalues by 
          using search_list function *)
@@ -388,22 +393,22 @@ Module Encschulze (Import C : Cand) (Import K : Keys) (Import Crp : CryptoAxioms
          it fetches the cth column of v and permute them by pi, so t c is 
          permuted cth column of v. Important *)
       remember (fun c =>
-                  shuffle grp (List.length cand_all)
+                  shuffle Crp.grp (List.length cand_all)
                           cand_all dec_cand (fun d => v d c) pi (rcolfunvalues c)) as t. 
       remember (fun c d => t d c) as w. (* transpose t to get w in row form *)
         
       (* construct zero knowledge proof of shuffle that w is column permutation of v by pi *)
       remember (fun c =>
-                  shuffle_zkp grp (List.length cand_all)
+                  shuffle_zkp Crp.grp (List.length cand_all)
                               cand_all (fun d => v d c) (fun d => w d c) pi cpi s (rcolfunvalues c))
         as zkppermvw.
       
-      assert (Ht2 : forall c, verify_col_permutation_ballot grp v w cpi zkppermvw c = true).
+      assert (Ht2 : forall c, verify_col_permutation_ballot Crp.grp v w cpi zkppermvw c = true).
       intros. unfold verify_col_permutation_ballot. 
       pose proof (verify_shuffle_axiom pi cpi s (fun d => v d c) (fun d => w d c)
                                        (rcolfunvalues c) (zkppermvw c)  Heqcpi).
       rewrite Heqw in H2.
-      assert ((fun d => t c d) = shuffle grp (List.length cand_all)
+      assert ((fun d => t c d) = shuffle Crp.grp (List.length cand_all)
                                       cand_all dec_cand (fun d : cand => v d c) pi (rcolfunvalues c)).
       rewrite Heqt; try auto.
       specialize (H2 H3).
@@ -412,13 +417,13 @@ Module Encschulze (Import C : Cand) (Import K : Keys) (Import Crp : CryptoAxioms
 
       
       (* Now decrypt the ballot w. *)
-      remember (fun c d => decrypt_message grp privatekey (w c d)) as b.
+      remember (fun c d => decrypt_message Crp.grp privatekey (w c d)) as b.
       (* construct zero knowledge proof of decryption *)
       remember (fun c d => construct_zero_knowledge_decryption_proof
-                          grp privatekey (w c d)) as zkpdecw.
+                          Crp.grp privatekey (w c d)) as zkpdecw.
       (* Show that the zkpdecw is true b is honest decryption of w *)
       assert (Ht3 : forall c d, verify_zero_knowledge_decryption_proof
-                              grp (b c d) (w c d) (zkpdecw c d) = true).
+                              Crp.grp (b c d) (w c d) (zkpdecw c d) = true).
       intros c d. rewrite Heqzkpdecw.
       apply verify_honest_decryption_zkp. rewrite Heqb. reflexivity.
 
@@ -428,12 +433,12 @@ Module Encschulze (Import C : Cand) (Import K : Keys) (Import Crp : CryptoAxioms
          If b is not valid then it contains cycle and this reflects back to u *)
       destruct (matrix_ballot_valid_dec b) as [Hb | Hnb].
       (* Since b is valid so add the ballot u to margin m and call it nm *)
-      remember (fun c d => homomorphic_addition grp (u c d) (m c d)) as nm.
-      assert (Ht4 : forall c d, nm c d = homomorphic_addition grp (u c d) (m c d)).
+      remember (fun c d => homomorphic_addition Crp.grp (u c d) (m c d)) as nm.
+      assert (Ht4 : forall c d, nm c d = homomorphic_addition Crp.grp (u c d) (m c d)).
       intros c d.  rewrite Heqnm. reflexivity.
       
       (* ecvalid *) 
-      pose proof (ecvalid grp bs u v w b zkppermuv zkppermvw
+      pose proof (ecvalid Crp.grp bs u v w b zkppermuv zkppermvw
                           zkpdecw cpi zkpcpi ts m nm inbs He
                           Hb H Ht1 Ht2 Ht3 Ht4).
       (* Induction Hypothesis *)
@@ -441,7 +446,7 @@ Module Encschulze (Import C : Cand) (Import K : Keys) (Import Crp : CryptoAxioms
       exists inb, mrg. assumption.
  
       (* ecinvalid *)
-      pose proof (ecinvalid grp bs u v w b zkppermuv zkppermvw
+      pose proof (ecinvalid Crp.grp bs u v w b zkppermuv zkppermvw
                             zkpdecw cpi zkpcpi ts m inbs He Hnb H
                             Ht1 Ht2 Ht3).
       destruct (IHs (u :: inbs) m X) as [inb [mrg T]].
@@ -455,7 +460,7 @@ Module Encschulze (Import C : Cand) (Import K : Keys) (Import Crp : CryptoAxioms
      (* for every list of incoming ballots, we can progress the count to a state where all
      ballots are processed *)
     Lemma  pall_ballots_counted (bs : list eballot) :
-      existsT i m, ECount grp bs (epartial ([], i) m).
+      existsT i m, ECount Crp.grp bs (epartial ([], i) m).
     Proof.
       pose proof (ecount_all_ballot bs) as Hs.
       destruct Hs as [encm Heg].
@@ -467,13 +472,13 @@ Module Encschulze (Import C : Cand) (Import K : Keys) (Import Crp : CryptoAxioms
       
     (* We decrypt the encrypted margin to run the computation *)
     Lemma decrypt_margin (bs : list eballot) :
-      existsT m, ECount grp bs (edecrypt m).
+      existsT m, ECount Crp.grp bs (edecrypt m).
     Proof.
       remember (pall_ballots_counted bs) as Hc.
       destruct Hc as [i [m Hcount]].
-      remember (fun c d => decrypt_message grp privatekey (m c d)) as decm.
+      remember (fun c d => decrypt_message Crp.grp privatekey (m c d)) as decm.
       remember (fun c d => construct_zero_knowledge_decryption_proof
-                          grp privatekey (m c d)) as zkpdecm. 
+                          Crp.grp privatekey (m c d)) as zkpdecm. 
       exists decm.
       apply ecdecrypt with (inbs := i) (encm := m) (zkp := zkpdecm). 
       assumption.
@@ -485,12 +490,12 @@ Module Encschulze (Import C : Cand) (Import K : Keys) (Import Crp : CryptoAxioms
     (* The main theorem: for every list of ballots, we can find a boolean function that decides
      winners, together with evidences of the correctness of this determination *)
     Lemma pschulze_winners (bs : list eballot) :
-      existsT (f : cand -> bool), ECount grp bs (ewinners f).
+      existsT (f : cand -> bool), ECount Crp.grp bs (ewinners f).
     Proof.
       destruct (decrypt_margin bs) as [dm Hecount].
-      exists (c_wins dm).
-      pose proof (ecfin grp bs dm (c_wins dm) (wins_loses_type_dec dm) Hecount).
-      pose proof (X (c_wins_true_type dm) (c_wins_false_type dm)).
+      exists (M.c_wins dm).
+      pose proof (ecfin Crp.grp bs dm (M.c_wins dm) (M.wins_loses_type_dec dm) Hecount).
+      pose proof (X (M.c_wins_true_type dm) (M.c_wins_false_type dm)).
       auto.
     Defined.
 
@@ -501,7 +506,7 @@ Module Encschulze (Import C : Cand) (Import K : Keys) (Import Crp : CryptoAxioms
        pschulze_winners are same if ballots match *)
     
     (* This function connects ballot ot pballot *)
-    Definition map_ballot_pballot (b : ballot) (p : pballot) :=
+    Definition map_ballot_pballot (b : M.ballot) (p : pballot) :=
       ((exists c,  b c = 0)%nat /\ ~matrix_ballot_valid p) \/
       (matrix_ballot_valid p /\ (forall c, b c > 0)%nat /\
        (forall c d, (p c d = 1 <-> (b c < b d)%nat) /\
@@ -511,7 +516,7 @@ Module Encschulze (Import C : Cand) (Import K : Keys) (Import Crp : CryptoAxioms
     
     (* This reason I am going with this proof is that my proofs depends on this. 
        But inductive type is more elegant *)
-    Fixpoint mapping_ballot_pballot (bs : list ballot) (pbs : list pballot) : Prop. 
+    Fixpoint mapping_ballot_pballot (bs : list M.ballot) (pbs : list pballot) : Prop. 
     Proof.
       refine (match bs, pbs with
               | [], [] => True
@@ -524,16 +529,16 @@ Module Encschulze (Import C : Cand) (Import K : Keys) (Import Crp : CryptoAxioms
     Defined.
 
     Lemma connect_validity_of_ballot_pballot :
-      forall (b : ballot) (p : pballot),
+      forall (b : M.ballot) (p : pballot),
         map_ballot_pballot b p -> 
-        proj1_sig (bool_of_sumbool (ballot_valid_dec b)) = true <->
+        proj1_sig (bool_of_sumbool (M.ballot_valid_dec b)) = true <->
         proj1_sig (bool_of_sumbool (matrix_ballot_valid_dec p)) = true.
     Proof.
       intros b p H.
       split; intros.
       unfold map_ballot_pballot in H. destruct H.
       destruct H.  destruct H as [c H].
-      destruct (bool_of_sumbool (ballot_valid_dec b)).
+      destruct (bool_of_sumbool (M.ballot_valid_dec b)).
       simpl in H0. rewrite H0 in y.  pose proof (y c).  omega.
       destruct H as [H1 [H2 H3]].
       destruct (bool_of_sumbool (matrix_ballot_valid_dec p)).
@@ -544,14 +549,14 @@ Module Encschulze (Import C : Cand) (Import K : Keys) (Import Crp : CryptoAxioms
       destruct (bool_of_sumbool (matrix_ballot_valid_dec p)). simpl in *.
       rewrite H0 in y. congruence.
       destruct H as [H1 [H2 H3]].
-      destruct (bool_of_sumbool (ballot_valid_dec b)). simpl in *.
+      destruct (bool_of_sumbool (M.ballot_valid_dec b)). simpl in *.
       destruct x.  auto. destruct y. pose proof (H2 x). omega.
     Qed.
 
     Lemma connect_invalidity_of_ballot_pballot :
-      forall (b : ballot) (p : pballot),
+      forall (b : M.ballot) (p : pballot),
         map_ballot_pballot b p -> 
-        proj1_sig (bool_of_sumbool (ballot_valid_dec b)) = false <->
+        proj1_sig (bool_of_sumbool (M.ballot_valid_dec b)) = false <->
         proj1_sig (bool_of_sumbool (matrix_ballot_valid_dec p)) = false.
     Proof.
       intros b p H.
@@ -561,12 +566,12 @@ Module Encschulze (Import C : Cand) (Import K : Keys) (Import Crp : CryptoAxioms
       destruct (bool_of_sumbool (matrix_ballot_valid_dec p)).
       simpl in *. destruct x; congruence.
       destruct H. destruct H1.
-      destruct (bool_of_sumbool (ballot_valid_dec b)). simpl in *.
+      destruct (bool_of_sumbool (M.ballot_valid_dec b)). simpl in *.
       rewrite H0 in y. destruct y.  pose proof (H1 x0). omega.
 
       unfold map_ballot_pballot in H.
       destruct H. destruct H. destruct H as [c H].
-      destruct (bool_of_sumbool (ballot_valid_dec b)). simpl in *.
+      destruct (bool_of_sumbool (M.ballot_valid_dec b)). simpl in *.
       destruct x. pose proof (y c). omega. auto.
       destruct H. destruct H1.
       destruct (bool_of_sumbool (matrix_ballot_valid_dec p)).
@@ -577,38 +582,38 @@ Module Encschulze (Import C : Cand) (Import K : Keys) (Import Crp : CryptoAxioms
    
   
     Lemma margin_same_from_both_existential 
-          (bs : list ballot) (ebs : list eballot) (pbs : list pballot)
-          (Ht : pbs = map (fun x => (fun c d => decrypt_message grp privatekey (x c d))) ebs)
+          (bs : list M.ballot) (ebs : list eballot) (pbs : list pballot)
+          (Ht : pbs = map (fun x => (fun c d => decrypt_message Crp.grp privatekey (x c d))) ebs)
           (H1 : mapping_ballot_pballot bs pbs) :
-      forall (s : State),
-        Count bs s ->
-        forall (ts : list ballot) (tinbs : list ballot)
+      forall (s : M.State),
+        M.Count bs s ->
+        forall (ts : list M.ballot) (tinbs : list M.ballot)
           (m : cand -> cand -> Z), (* valid ballot, invalid ballot, running margin *)
-          s = partial (ts, tinbs) m ->
+          s = M.partial (ts, tinbs) m ->
           existsT 
             (ets : list eballot) (etinbs : list eballot)
             (tpbs : list pballot) (etpbs : list pballot)
             (em : cand -> cand -> ciphertext),
-      (ECount grp ebs (epartial (ets, etinbs) em) *
-       (m = fun c d => decrypt_message grp privatekey (em c d)) *
-       (tpbs =  map (fun x => (fun c d => decrypt_message grp privatekey (x c d))) ets) *
-       (etpbs =  map (fun x => (fun c d => decrypt_message grp privatekey (x c d))) etinbs) * 
+      (ECount Crp.grp ebs (epartial (ets, etinbs) em) *
+       (m = fun c d => decrypt_message Crp.grp privatekey (em c d)) *
+       (tpbs =  map (fun x => (fun c d => decrypt_message Crp.grp privatekey (x c d))) ets) *
+       (etpbs =  map (fun x => (fun c d => decrypt_message Crp.grp privatekey (x c d))) etinbs) * 
        mapping_ballot_pballot ts tpbs *
        mapping_ballot_pballot tinbs etpbs)%type.
     Proof.   
       intros s H.  
       (* induction on structure of H *)
       induction H. intros. inversion H.
-      remember (fun c d => encrypt_message grp (m c d)) as em.
+      remember (fun c d => encrypt_message Crp.grp (m c d)) as em.
       exists ebs, [], pbs, [], em.
-      pose proof (ecax grp ebs ebs em m
+      pose proof (ecax Crp.grp ebs ebs em m
                        (fun c d => construct_zero_knowledge_decryption_proof
-                                  grp privatekey (em c d)) eq_refl e0).
+                                  Crp.grp privatekey (em c d)) eq_refl e0).
       simpl in X.
       assert (forall c d : cand,
                  verify_zero_knowledge_decryption_proof
-                   grp (m c d) (em c d)
-                   (construct_zero_knowledge_decryption_proof grp privatekey (em c d)) = true).
+                   Crp.grp (m c d) (em c d)
+                   (construct_zero_knowledge_decryption_proof Crp.grp privatekey (em c d)) = true).
       intros. subst. apply verify_honest_decryption_zkp. rewrite decryption_deterministic. auto.
       specialize (X H0). clear H0.
       repeat split. assumption.
@@ -647,21 +652,21 @@ Module Encschulze (Import C : Cand) (Import K : Keys) (Import Crp : CryptoAxioms
       rewrite Hets' in e1. 
       (*  ECount grp ebs (epartial (en :: ets', etinbs) em) 
           and u is valid then t is valid and it's encryption is valid *)
-      pose proof (ecvalid grp ebs).
+      pose proof (ecvalid Crp.grp ebs).
       (* u = en, v = row permutation of u, w is column permutation of v *)
       (* generate permutation *)  
-      remember (generatePermutation grp (List.length cand_all) cand_all) as pi.
+      remember (generatePermutation Crp.grp (List.length cand_all) cand_all) as pi.
       (* generate randomness S *)
-      remember  (generateS grp (List.length cand_all)) as s.
+      remember  (generateS Crp.grp (List.length cand_all)) as s.
       (* commit it *)
-      remember (generatePermutationCommitment grp (List.length cand_all) cand_all pi s) as cpi.
+      remember (generatePermutationCommitment Crp.grp (List.length cand_all) cand_all pi s) as cpi.
       (* generate zero knowledge proof of commitment *)
-      remember (zkpPermutationCommitment grp (List.length cand_all)
+      remember (zkpPermutationCommitment Crp.grp (List.length cand_all)
                                          cand_all pi cpi s) as zkpcpi. 
       (* At this point I can assert that 
          verify_permutation_commitment grp (List.length cand_all) cpi zkpcpi = true 
          using the Axiom permutation_commitment_axiom *)
-      assert (verify_permutation_commitment grp (List.length cand_all) cpi zkpcpi = true).
+      assert (verify_permutation_commitment Crp.grp (List.length cand_all) cpi zkpcpi = true).
       pose proof (permutation_commitment_axiom
                      pi cpi s zkpcpi Heqcpi Heqzkpcpi). auto.
 
@@ -670,7 +675,7 @@ Module Encschulze (Import C : Cand) (Import K : Keys) (Import Crp : CryptoAxioms
       (* Convert en -> rowpermute pi -> v *)
       (* What if i separate the R from shuffle ? *)
       (* This is what I am doing *)
-      remember (map (fun _ => generateR grp (List.length cand_all)) cand_all) as rrowlistvalues.
+      remember (map (fun _ => generateR Crp.grp (List.length cand_all)) cand_all) as rrowlistvalues.
       (* I have generated the randomness for each row and use them in shuffling. 
          It would be good idea to convert rlistvalues to rfunvalues by 
          using search_list function *)
@@ -683,12 +688,12 @@ Module Encschulze (Import C : Cand) (Import K : Keys) (Import Crp : CryptoAxioms
          in Shuffle *)
       (* get the ballot v by shuffling each row by pi and randomness R *)
       remember (fun c =>
-                  shuffle grp (List.length cand_all)
+                  shuffle Crp.grp (List.length cand_all)
                           cand_all dec_cand (en c) pi (rrowfunvalues c)) as v.
       (* construct zero knowledge proof of shuffle that v is row shuffle of u by pi
          using the same randomness R which used in shuffle *)
       remember (fun c =>
-                  shuffle_zkp grp (List.length cand_all)
+                  shuffle_zkp Crp.grp (List.length cand_all)
                               cand_all (en c) (v c) pi cpi s (rrowfunvalues c)) as zkppermuv.
       
       
@@ -696,11 +701,11 @@ Module Encschulze (Import C : Cand) (Import K : Keys) (Import Crp : CryptoAxioms
          The property here is construct matrix from u and v and comp
          This is bit tricky so I am leaving it for the moment because we need to 
          massage the axioms *)
-      assert (Ht1 : forall c, verify_row_permutation_ballot grp en v cpi zkppermuv c = true). 
+      assert (Ht1 : forall c, verify_row_permutation_ballot Crp.grp en v cpi zkppermuv c = true). 
       intros; unfold verify_row_permutation_ballot.
       pose proof (verify_shuffle_axiom pi cpi s (en c) (v c) (rrowfunvalues c) (zkppermuv c)
                                        Heqcpi).
-      assert (Hvr : v c = shuffle grp (List.length cand_all)
+      assert (Hvr : v c = shuffle Crp.grp (List.length cand_all)
                                   cand_all dec_cand (en c) pi (rrowfunvalues c)).
       rewrite Heqv; try auto.
       specialize (H11 Hvr). clear Hvr. rewrite Heqzkppermuv in H11.
@@ -709,7 +714,7 @@ Module Encschulze (Import C : Cand) (Import K : Keys) (Import Crp : CryptoAxioms
       
 
        (* generate again the randomness R to make sure that cryptographic sprit is high *)
-      remember (map (fun _ => generateR grp (List.length cand_all)) cand_all) as rcollistvalues.
+      remember (map (fun _ => generateR Crp.grp (List.length cand_all)) cand_all) as rcollistvalues.
       (* I have generated the randomness for each column and use them in shuffling. 
          It would be good idea to convert rcollistvalues to rcolfunvalues by 
          using search_list function *)
@@ -724,22 +729,22 @@ Module Encschulze (Import C : Cand) (Import K : Keys) (Import Crp : CryptoAxioms
          it fetches the cth column of v and permute them by pi, so t c is 
          permuted cth column of v. Important *)
       remember (fun c =>
-                  shuffle grp (List.length cand_all)
+                  shuffle Crp.grp (List.length cand_all)
                           cand_all dec_cand (fun d => v d c) pi (rcolfunvalues c)) as tt. 
       remember (fun c d => tt d c) as w. (* transpose t to get w in row form *)
         
       (* construct zero knowledge proof of shuffle that w is column permutation of v by pi *)
       remember (fun c =>
-                  shuffle_zkp grp (List.length cand_all)
+                  shuffle_zkp Crp.grp (List.length cand_all)
                               cand_all (fun d => v d c) (fun d => w d c) pi cpi s (rcolfunvalues c))
         as zkppermvw.
       
-      assert (Ht2 : forall c, verify_col_permutation_ballot grp v w cpi zkppermvw c = true).
+      assert (Ht2 : forall c, verify_col_permutation_ballot Crp.grp v w cpi zkppermvw c = true).
       intros. unfold verify_col_permutation_ballot. 
       pose proof (verify_shuffle_axiom pi cpi s (fun d => v d c) (fun d => w d c)
                                        (rcolfunvalues c) (zkppermvw c)  Heqcpi).
       rewrite Heqw in H12.
-      assert ((fun d => tt c d) = shuffle grp (List.length cand_all)
+      assert ((fun d => tt c d) = shuffle Crp.grp (List.length cand_all)
                                        cand_all dec_cand (fun d : cand => v d c) pi (rcolfunvalues c)).
       rewrite Heqtt; try auto.
       specialize (H12 H13).
@@ -749,13 +754,13 @@ Module Encschulze (Import C : Cand) (Import K : Keys) (Import Crp : CryptoAxioms
 
       
       (* Now decrypt the ballot w *)
-      remember (fun c d => decrypt_message grp privatekey (w c d)) as b.
+      remember (fun c d => decrypt_message Crp.grp privatekey (w c d)) as b.
       (* construct zero knowledge proof of decryption *)
       remember (fun c d => construct_zero_knowledge_decryption_proof
-                          grp privatekey (w c d)) as zkpdecw.
+                          Crp.grp privatekey (w c d)) as zkpdecw.
       (* Show that the zkpdecw is true b is honest decryption of w *)
       assert (Ht3 : forall c d, verify_zero_knowledge_decryption_proof
-                              grp (b c d) (w c d) (zkpdecw c d) = true).
+                              Crp.grp (b c d) (w c d) (zkpdecw c d) = true).
       intros c d. rewrite Heqzkpdecw.
       apply verify_honest_decryption_zkp. rewrite Heqb. reflexivity.
       
@@ -768,7 +773,7 @@ Module Encschulze (Import C : Cand) (Import K : Keys) (Import Crp : CryptoAxioms
       pose proof (proj1 (connect_validity_of_ballot_pballot u t H2)). 
       (* I know that u is valid (Hypothesis g) *)
       assert (proj1_sig (bool_of_sumbool (matrix_ballot_valid_dec t)) = true).
-      destruct (ballot_valid_dec u). simpl in H12. 
+      destruct (M.ballot_valid_dec u). simpl in H12. 
       specialize (H12 eq_refl). auto.
       destruct e0. pose proof (g x). omega.
       clear H12. destruct (matrix_ballot_valid_dec t); swap 1 2.
@@ -780,25 +785,25 @@ Module Encschulze (Import C : Cand) (Import K : Keys) (Import Crp : CryptoAxioms
       destruct pi as [pi Sig].
       
       (* Each row of v is shuffle of each row of en by permutation pi *)      
-      assert (forall c d, t c d = decrypt_message grp privatekey (en c d)).
+      assert (forall c d, t c d = decrypt_message Crp.grp privatekey (en c d)).
       intros. rewrite H6. auto.
 
       (* Interpretation of permutation. v c d = en c (pi d) and it means 
          that element at '(pi d)' position in cth row of en goes to 'd' position of cth row in v *) 
-      assert (forall c d, decrypt_message grp privatekey (v c d) =
-                     decrypt_message grp privatekey (en c (pi d))). 
+      assert (forall c d, decrypt_message Crp.grp privatekey (v c d) =
+                     decrypt_message Crp.grp privatekey (en c (pi d))). 
       rewrite Heqv. intros. 
-      assert (shuffle grp (List.length cand_all) cand_all dec_cand (en c)
+      assert (shuffle Crp.grp (List.length cand_all) cand_all dec_cand (en c)
                       (existT (fun pi : cand -> cand => Bijective pi) pi Sig) (rrowfunvalues c) = v c).
       rewrite Heqv. auto.
       rewrite H13. eapply shuffle_perm in H13. 
       unfold compose in H13.
       instantiate (1 := d) in H13. simpl in H13. assumption.
 
-      assert (forall c d, decrypt_message grp privatekey (w c d) =
-                     decrypt_message grp privatekey (v (pi c) d)).  
+      assert (forall c d, decrypt_message Crp.grp privatekey (w c d) =
+                     decrypt_message Crp.grp privatekey (v (pi c) d)).  
       rewrite Heqw. intros. rewrite Heqtt.
-      assert (shuffle grp (List.length cand_all) cand_all dec_cand (fun d0 : cand => v d0 d)
+      assert (shuffle Crp.grp (List.length cand_all) cand_all dec_cand (fun d0 : cand => v d0 d)
                       (existT (fun pi0 : cand -> cand => Bijective pi0) pi Sig) (rcolfunvalues d) =
               fun d0 => w d0 d).
       rewrite Heqw. rewrite Heqtt. auto.
@@ -806,8 +811,8 @@ Module Encschulze (Import C : Cand) (Import K : Keys) (Import Crp : CryptoAxioms
       unfold compose in H14.
       instantiate (1 := c) in H14. cbn in H14. auto.
 
-      assert (forall c d, decrypt_message grp privatekey (w c d) =
-                     decrypt_message grp privatekey (en (pi c) (pi d))).
+      assert (forall c d, decrypt_message Crp.grp privatekey (w c d) =
+                     decrypt_message Crp.grp privatekey (en (pi c) (pi d))).
       intros. rewrite  H14. rewrite H13. auto.
      
 
@@ -826,17 +831,17 @@ Module Encschulze (Import C : Cand) (Import K : Keys) (Import Crp : CryptoAxioms
       specialize (X en v w b zkppermuv zkppermvw zkpdecw cpi
                     zkpcpi ets' em
                     (fun c d : cand => homomorphic_addition
-                                      grp (en c d) (em c d))
+                                      Crp.grp (en c d) (em c d))
                     etinbs e1 H12 H9 Ht1 Ht2 Ht3).
       simpl in X.
       assert ((forall c d : cand,
-                  homomorphic_addition grp (en c d) (em c d) =
-                  homomorphic_addition grp (en c d) (em c d))).
+                  homomorphic_addition Crp.grp (en c d) (em c d) =
+                  homomorphic_addition Crp.grp (en c d) (em c d))).
       auto.
       specialize (X H13).
       (*  ECount grp ebs
         (epartial (ets', etinbs) (fun c d : cand => homomorphic_addition grp (en c d) (em c d))) *)
-      exists ets', etinbs, tbps', etpbs, (fun c d : cand => homomorphic_addition grp (en c d) (em c d)).
+      exists ets', etinbs, tbps', etpbs, (fun c d : cand => homomorphic_addition Crp.grp (en c d) (em c d)).
       repeat split. auto. 
       apply functional_extensionality. intros.
       apply functional_extensionality. intros.
@@ -844,9 +849,9 @@ Module Encschulze (Import C : Cand) (Import K : Keys) (Import Crp : CryptoAxioms
       rewrite H14.
       (*  m = (fun c d : cand => decrypt_message grp privatekey (em c d))
            H6 : t = (fun c d : cand => decrypt_message grp privatekey (en c d)) *)
-      assert (t x x0 = decrypt_message grp privatekey (en x x0)).
+      assert (t x x0 = decrypt_message Crp.grp privatekey (en x x0)).
       rewrite H6. auto.
-      assert (m x x0 = decrypt_message grp privatekey (em x x0)).
+      assert (m x x0 = decrypt_message Crp.grp privatekey (em x x0)).
       rewrite e2. auto.
       rewrite <- H15. rewrite <- H16.
       rewrite <- H5.
@@ -867,15 +872,15 @@ Module Encschulze (Import C : Cand) (Import K : Keys) (Import Crp : CryptoAxioms
       apply H2cdt1 in Hul. rewrite Hul. omega.
       pose proof (H18 Hul). apply H2cdt2 in Hul. rewrite Hul. omega.
       assert (u x > u x0)%nat by omega.
-      pose proof (H19 H2). apply H2cdt3 in H2. rewrite H2.  omega.
+      pose proof (H19 H2). apply H2cdt3 in H2. rewrite H2. omega.
       assumption. assumption. rewrite H3 in H8. assumption.
       rewrite H4 in m1. assumption.
       (* Wohoo. Valid case discharged. *)
 
       (* Now we are in situation where u is not valid. *)
       intros. inversion H0.
-      assert (proj1_sig (bool_of_sumbool (ballot_valid_dec u)) = false).
-      destruct (ballot_valid_dec u); simpl; try auto.
+      assert (proj1_sig (bool_of_sumbool (M.ballot_valid_dec u)) = false).
+      destruct (M.ballot_valid_dec u); simpl; try auto.
       destruct e as [c Hc]. pose proof (g c). omega.
 
       assert (forall (A : Type) (l : list A),
@@ -909,18 +914,18 @@ Module Encschulze (Import C : Cand) (Import K : Keys) (Import Crp : CryptoAxioms
       (* ecinvalid *)
 
       (* generate permutation *)  
-      remember (generatePermutation grp (List.length cand_all) cand_all) as pi.
+      remember (generatePermutation Crp.grp (List.length cand_all) cand_all) as pi.
       (* generate randomness S *)
-      remember (generateS grp (List.length cand_all)) as s.
+      remember (generateS Crp.grp (List.length cand_all)) as s.
       (* commit it *)
-      remember (generatePermutationCommitment grp (List.length cand_all) cand_all pi s) as cpi.
+      remember (generatePermutationCommitment Crp.grp (List.length cand_all) cand_all pi s) as cpi.
       (* generate zero knowledge proof of commitment *)
-      remember (zkpPermutationCommitment grp (List.length cand_all)
+      remember (zkpPermutationCommitment Crp.grp (List.length cand_all)
                                          cand_all pi cpi s) as zkpcpi. 
       (* At this point I can assert that 
          verify_permutation_commitment grp (List.length cand_all) cpi zkpcpi = true 
          using the Axiom permutation_commitment_axiom *)
-      assert (verify_permutation_commitment grp (List.length cand_all) cpi zkpcpi = true).
+      assert (verify_permutation_commitment Crp.grp (List.length cand_all) cpi zkpcpi = true).
       pose proof (permutation_commitment_axiom
                     pi cpi s zkpcpi Heqcpi Heqzkpcpi). auto.
 
@@ -928,7 +933,7 @@ Module Encschulze (Import C : Cand) (Import K : Keys) (Import Crp : CryptoAxioms
       (* Convert en -> rowpermute pi -> v *)
       (* What if i separate the R from shuffle ? *)
       (* This is what I am doing *)
-      remember (map (fun _ => generateR grp (List.length cand_all)) cand_all) as rrowlistvalues.
+      remember (map (fun _ => generateR Crp.grp (List.length cand_all)) cand_all) as rrowlistvalues.
       (* I have generated the randomness for each row and use them in shuffling. 
          It would be good idea to convert rlistvalues to rfunvalues by 
          using search_list function *)
@@ -941,12 +946,12 @@ Module Encschulze (Import C : Cand) (Import K : Keys) (Import Crp : CryptoAxioms
          in Shuffle *)
       (* get the ballot v by shuffling each row by pi and randomness R *)
       remember (fun c =>
-                  shuffle grp (List.length cand_all)
+                  shuffle Crp.grp (List.length cand_all)
                           cand_all dec_cand (en c) pi (rrowfunvalues c)) as v.
       (* construct zero knowledge proof of shuffle that v is row shuffle of u by pi
          using the same randomness R which used in shuffle *)
       remember (fun c =>
-                  shuffle_zkp grp (List.length cand_all)
+                  shuffle_zkp Crp.grp (List.length cand_all)
                               cand_all (en c) (v c) pi cpi s (rrowfunvalues c)) as zkppermuv.
       
            
@@ -954,11 +959,11 @@ Module Encschulze (Import C : Cand) (Import K : Keys) (Import Crp : CryptoAxioms
          The property here is construct matrix from u and v and comp
          This is bit tricky so I am leaving it for the moment because we need to 
          massage the axioms *)
-      assert (Ht1 : forall c, verify_row_permutation_ballot grp en v cpi zkppermuv c = true). 
+      assert (Ht1 : forall c, verify_row_permutation_ballot Crp.grp en v cpi zkppermuv c = true). 
       intros; unfold verify_row_permutation_ballot.
       pose proof (verify_shuffle_axiom pi cpi s (en c) (v c) (rrowfunvalues c) (zkppermuv c)
                                         Heqcpi).
-      assert (Hvr : v c = shuffle grp (List.length cand_all)
+      assert (Hvr : v c = shuffle Crp.grp (List.length cand_all)
                                   cand_all dec_cand (en c) pi (rrowfunvalues c)).
       rewrite Heqv; try auto.
       specialize (H14 Hvr). clear Hvr. rewrite Heqzkppermuv in H14.
@@ -967,7 +972,7 @@ Module Encschulze (Import C : Cand) (Import K : Keys) (Import Crp : CryptoAxioms
 
 
        (* generate again the randomness R to make sure that cryptographic sprit is high *)
-      remember (map (fun _ => generateR grp (List.length cand_all)) cand_all) as rcollistvalues.
+      remember (map (fun _ => generateR Crp.grp (List.length cand_all)) cand_all) as rcollistvalues.
       (* I have generated the randomness for each column and use them in shuffling. 
          It would be good idea to convert rcollistvalues to rcolfunvalues by 
          using search_list function *)
@@ -982,22 +987,22 @@ Module Encschulze (Import C : Cand) (Import K : Keys) (Import Crp : CryptoAxioms
          it fetches the cth column of v and permute them by pi, so t c is 
          permuted cth column of v. Important *)
       remember (fun c =>
-                  shuffle grp (List.length cand_all)
+                  shuffle Crp.grp (List.length cand_all)
                           cand_all dec_cand (fun d => v d c) pi (rcolfunvalues c)) as tt. 
       remember (fun c d => tt d c) as w. (* transpose t to get w in row form *)
         
       (* construct zero knowledge proof of shuffle that w is column permutation of v by pi *)
       remember (fun c =>
-                  shuffle_zkp grp (List.length cand_all)
+                  shuffle_zkp Crp.grp (List.length cand_all)
                               cand_all (fun d => v d c) (fun d => w d c) pi cpi s (rcolfunvalues c))
         as zkppermvw.
       
-      assert (Ht2 : forall c, verify_col_permutation_ballot grp v w cpi zkppermvw c = true).
+      assert (Ht2 : forall c, verify_col_permutation_ballot Crp.grp v w cpi zkppermvw c = true).
       intros. unfold verify_col_permutation_ballot. 
       pose proof (verify_shuffle_axiom pi cpi s (fun d => v d c) (fun d => w d c)
                                        (rcolfunvalues c) (zkppermvw c)  Heqcpi).
       rewrite Heqw in H15.
-      assert ((fun d => tt c d) = shuffle grp (List.length cand_all)
+      assert ((fun d => tt c d) = shuffle Crp.grp (List.length cand_all)
                                       cand_all dec_cand (fun d : cand => v d c) pi (rcolfunvalues c)).
       rewrite Heqtt; try auto.
       specialize (H15 H16).
@@ -1006,13 +1011,13 @@ Module Encschulze (Import C : Cand) (Import K : Keys) (Import Crp : CryptoAxioms
 
       
       (* Now decrypt the ballot w *)
-      remember (fun c d => decrypt_message grp privatekey (w c d)) as b.
+      remember (fun c d => decrypt_message Crp.grp privatekey (w c d)) as b.
       (* construct zero knowledge proof of decryption *)
       remember (fun c d => construct_zero_knowledge_decryption_proof
-                          grp privatekey (w c d)) as zkpdecw.
+                          Crp.grp privatekey (w c d)) as zkpdecw.
       (* Show that the zkpdecw is true b is honest decryption of w *)
       assert (Ht3 : forall c d, verify_zero_knowledge_decryption_proof
-                              grp (b c d) (w c d) (zkpdecw c d) = true).
+                              Crp.grp (b c d) (w c d) (zkpdecw c d) = true).
       intros c d. rewrite Heqzkpdecw.
       apply verify_honest_decryption_zkp. rewrite Heqb. reflexivity. 
       (* At this point we need Axioms which connects the validity of en to b 
@@ -1021,8 +1026,8 @@ Module Encschulze (Import C : Cand) (Import K : Keys) (Import Crp : CryptoAxioms
          H11 : tp = (fun c d : cand => decrypt_message grp privatekey (en c d))
          u is invalid and it infers that t is also invalid. 
          t is invalid then it's encryption en is also invalid *)
-      assert (proj1_sig (bool_of_sumbool (ballot_valid_dec u)) = false).
-      destruct (bool_of_sumbool (ballot_valid_dec u)). simpl.
+      assert (proj1_sig (bool_of_sumbool (M.ballot_valid_dec u)) = false).
+      destruct (bool_of_sumbool (M.ballot_valid_dec u)). simpl.
       destruct x. destruct e as [e Hc]. pose proof (y e). omega.
       auto.
       pose proof (proj1 (connect_invalidity_of_ballot_pballot u tp H6) H15).
@@ -1040,24 +1045,24 @@ Module Encschulze (Import C : Cand) (Import K : Keys) (Import Crp : CryptoAxioms
       destruct pi as [pi Sig]. 
       (* Each row of v is shuffle of each row of en by permutation pi *)
       
-      assert (forall c d, tp c d = decrypt_message grp privatekey (en c d)).
+      assert (forall c d, tp c d = decrypt_message Crp.grp privatekey (en c d)).
       intros. rewrite H11. auto.
 
 
-      assert (forall c d, decrypt_message grp privatekey (v c d) =
-                     decrypt_message grp privatekey (en c (pi d))). 
+      assert (forall c d, decrypt_message Crp.grp privatekey (v c d) =
+                     decrypt_message Crp.grp privatekey (en c (pi d))). 
       rewrite Heqv. intros. 
-      assert (shuffle grp (List.length cand_all) cand_all dec_cand (en c)
+      assert (shuffle Crp.grp (List.length cand_all) cand_all dec_cand (en c)
                       (existT (fun pi : cand -> cand => Bijective pi) pi Sig) (rrowfunvalues c) = v c).
       rewrite Heqv. auto.
       rewrite H18. eapply shuffle_perm in H18. 
       unfold compose in H18.
       instantiate (1 := d) in H18. simpl in H18. assumption.
 
-      assert (forall c d, decrypt_message grp privatekey (w c d) =
-                     decrypt_message grp privatekey (v (pi c) d)).   
+      assert (forall c d, decrypt_message Crp.grp privatekey (w c d) =
+                     decrypt_message Crp.grp privatekey (v (pi c) d)).   
       rewrite Heqw. intros. rewrite Heqtt.
-      assert (shuffle grp (List.length cand_all ) cand_all dec_cand (fun d0 : cand => v d0 d)
+      assert (shuffle Crp.grp (List.length cand_all ) cand_all dec_cand (fun d0 : cand => v d0 d)
                       (existT (fun pi0 : cand -> cand => Bijective pi0) pi Sig) (rcolfunvalues d) =
               fun d0 => w d0 d).
       rewrite Heqw. rewrite Heqtt. auto.
@@ -1065,8 +1070,8 @@ Module Encschulze (Import C : Cand) (Import K : Keys) (Import Crp : CryptoAxioms
       unfold compose in H19.
       instantiate (1 := c) in H19. cbn in H19. auto.
 
-      assert (forall c d, decrypt_message grp privatekey (w c d) =
-                     decrypt_message grp privatekey (en (pi c) (pi d))).
+      assert (forall c d, decrypt_message Crp.grp privatekey (w c d) =
+                     decrypt_message Crp.grp privatekey (en (pi c) (pi d))).
       intros. rewrite  H19. rewrite H18. auto.
 
       
@@ -1087,7 +1092,7 @@ Module Encschulze (Import C : Cand) (Import K : Keys) (Import Crp : CryptoAxioms
       rewrite H21 in H22.  rewrite Hg2 in H22.
       rewrite Hg2 in H22. auto.
             
-      pose proof (ecinvalid grp ebs en v w b zkppermuv zkppermvw zkpdecw cpi
+      pose proof (ecinvalid Crp.grp ebs en v w b zkppermuv zkppermvw zkpdecw cpi
                             zkpcpi  ets' em etinbs He H18 H10 Ht1 Ht2 Ht3).
       exists ets', (en :: etinbs), tpbs', (tp :: etpbs), em.
       repeat split. assumption. rewrite <- H5. assumption.
@@ -1099,12 +1104,12 @@ Module Encschulze (Import C : Cand) (Import K : Keys) (Import Crp : CryptoAxioms
     Qed.   
     
     
-    Fixpoint compute_margin (bs : list ballot) :=
+    Fixpoint compute_margin (bs : list M.ballot) :=
       match bs with
       | [] => fun c d => 0
       | h :: t =>
-        match ballot_valid_dec h with
-        | left _ => update_marg h (compute_margin t)
+        match M.ballot_valid_dec h with
+        | left _ => M.update_marg h (compute_margin t)
         | right _ => compute_margin t
         end
       end.
@@ -1119,9 +1124,9 @@ Module Encschulze (Import C : Cand) (Import K : Keys) (Import Crp : CryptoAxioms
     
     Lemma compute_assoc :
       forall u a m, (forall c, u c > 0)%nat -> (forall c, a c > 0)%nat ->  
-               update_marg u (update_marg a m) = update_marg a (update_marg u m).
+               M.update_marg u (M.update_marg a m) = M.update_marg a (M.update_marg u m).
     Proof.
-      intros.  unfold update_marg.
+      intros.  unfold M.update_marg.
       apply functional_extensionality; intros.
       apply functional_extensionality; intros.
       destruct (nat_dec_me (u x) (u x0)) as [[H1 | H1] | H1].
@@ -1155,14 +1160,14 @@ Module Encschulze (Import C : Cand) (Import K : Keys) (Import Crp : CryptoAxioms
       
     
     Lemma valid_compute_margin_distributes :
-      forall bs (u : ballot), (forall c, u c > 0)%nat ->
-                         compute_margin (bs ++ [u]) = update_marg u (compute_margin bs).
+      forall bs (u : M.ballot), (forall c, u c > 0)%nat ->
+                         compute_margin (bs ++ [u]) = M.update_marg u (compute_margin bs).
     Proof.
       induction bs; simpl; intros; try auto.
-      destruct (ballot_valid_dec u). auto.
+      destruct (M.ballot_valid_dec u). auto.
       destruct e as [e He]. pose proof (H e). omega.
        
-      destruct (ballot_valid_dec a).
+      destruct (M.ballot_valid_dec a).
       rewrite (compute_assoc _ _ _ H g).
       specialize (IHbs u H). rewrite IHbs. auto.
       pose proof (IHbs u H). assumption.
@@ -1170,22 +1175,22 @@ Module Encschulze (Import C : Cand) (Import K : Keys) (Import Crp : CryptoAxioms
     
 
     Lemma invalid_compute_margin_same :
-      forall bs (u : ballot), (exists c, u c = 0)%nat -> compute_margin (bs ++ [u]) = compute_margin bs.
+      forall bs (u : M.ballot), (exists c, u c = 0)%nat -> compute_margin (bs ++ [u]) = compute_margin bs.
     Proof.
       induction bs; simpl; intros; try auto.
-      destruct (ballot_valid_dec u). destruct H as [e H].
+      destruct (M.ballot_valid_dec u). destruct H as [e H].
       pose proof (g e). omega. auto.
       
-      destruct (ballot_valid_dec a).
+      destruct (M.ballot_valid_dec a).
       pose proof (IHbs u H). rewrite H0. auto.
       pose proof (IHbs u H). auto.
     Qed.
       
 
     Lemma tail_count : forall bs s,
-        Count bs s ->
+        M.Count bs s ->
         forall us inbs m,
-          s = partial (us, inbs) m ->
+          s = M.partial (us, inbs) m ->
           exists cs', bs = cs' ++ us  /\ m = compute_margin cs'.
     Proof.
       (* This proof is for m = compute_margin cs' *)
@@ -1200,7 +1205,7 @@ Module Encschulze (Import C : Cand) (Import K : Keys) (Import Crp : CryptoAxioms
       destruct H as [cs' [H1 H2]].
       exists (cs' ++ [u]). split. rewrite app_assoc_reverse. auto.
       rewrite (valid_compute_margin_distributes _ _ g). rewrite <- H2. 
-      unfold update_marg. apply functional_extensionality; intros.
+      unfold M.update_marg. apply functional_extensionality; intros.
       apply functional_extensionality; intros. 
       destruct (a x x0) as [H3 [H4 H5]].
       destruct (lt_eq_lt_dec (u x) (u x0)) as [[H6 | H6] | H6].
@@ -1224,9 +1229,9 @@ Module Encschulze (Import C : Cand) (Import K : Keys) (Import Crp : CryptoAxioms
 
 
     (* Counting same list of ballots would give same margin *)
-    Lemma unique_margin : forall bs inbs inbs0 m m0 s s0 (c0 : Count bs s) (c1 : Count bs s0),
-        s = partial ([], inbs) m ->
-        s0 = partial ([], inbs0) m0 -> m = m0.
+    Lemma unique_margin : forall bs inbs inbs0 m m0 s s0 (c0 : M.Count bs s) (c1 : M.Count bs s0),
+        s = M.partial ([], inbs) m ->
+        s0 = M.partial ([], inbs0) m0 -> m = m0.
     Proof.
       intros.
       pose proof (tail_count bs s c0 [] inbs m H).
@@ -1241,7 +1246,7 @@ Module Encschulze (Import C : Cand) (Import K : Keys) (Import Crp : CryptoAxioms
                                                                             
     (* Uniqueness of winners *)
     Lemma uniqueness_proof : forall bs w w',
-        Count bs (winners w) -> Count bs (winners w') -> w = w'.
+        M.Count bs (M.winners w) -> M.Count bs (M.winners w') -> w = w'.
     Proof.
       intros bs w w' H1 H2.     
       inversion H1. inversion H2.
@@ -1256,22 +1261,22 @@ Module Encschulze (Import C : Cand) (Import K : Keys) (Import Crp : CryptoAxioms
       specialize ((proj1 H0) eq_refl); intros.
       destruct H. destruct H4.
       destruct H3. destruct H5.
-      pose proof (loses_type_prop m0 x x0).
-      pose proof (loses_prop_iterated_marg m0 x H9).
+      pose proof (M.loses_type_prop m0 x x0).
+      pose proof (M.loses_prop_iterated_marg m0 x H9).
       destruct H10 as [dd H10].
-      pose proof (wins_type_prop m0 x x1).
-      pose proof (wins_prop_iterated_marg m0 x H11).
+      pose proof (M.wins_type_prop m0 x x1).
+      pose proof (M.wins_prop_iterated_marg m0 x H11).
       pose proof (H12 dd). omega.
 
       specialize ((proj1 H3) eq_refl); intros.
       specialize ((proj1 H5) eq_refl); intros.
       destruct H. destruct H4.
       destruct H3. destruct H5.
-      pose proof (loses_type_prop m0 x x0).
-      pose proof (loses_prop_iterated_marg m0 x H9).
+      pose proof (M.loses_type_prop m0 x x0).
+      pose proof (M.loses_prop_iterated_marg m0 x H9).
       destruct H10 as [dd H10].
-      pose proof (wins_type_prop m0 x x1).
-      pose proof (wins_prop_iterated_marg m0 x H11).
+      pose proof (M.wins_type_prop m0 x x1).
+      pose proof (M.wins_prop_iterated_marg m0 x H11).
       pose proof (H12 dd). omega.
     Qed.
     
@@ -1280,15 +1285,15 @@ Module Encschulze (Import C : Cand) (Import K : Keys) (Import Crp : CryptoAxioms
     (* If there one to one correspondence between ballots and encrypted ballots, 
        then computing winners via plaintext ballot is same as encrypted ballot *)
     Lemma plaintext_schulze_to_homomorphic:
-    forall (bs : list ballot) (pbs : list pballot) (ebs : list eballot)
+    forall (bs : list M.ballot) (pbs : list pballot) (ebs : list eballot)
       (w : cand -> bool)
-      (H : pbs = map (fun x => (fun c d => decrypt_message grp privatekey (x c d))) ebs)
+      (H : pbs = map (fun x => (fun c d => decrypt_message Crp.grp privatekey (x c d))) ebs)
       (H2 : mapping_ballot_pballot bs pbs), (* valid b <-> valid pb *)
-      Count bs (winners w) -> ECount grp ebs (ewinners w).
+      M.Count bs (M.winners w) -> ECount Crp.grp ebs (ewinners w).
     Proof.
       (* Show that margin computed from bs is same as ebs *)
       intros bs pbs ebs w H0 H1 H2.
-      destruct (all_ballots_counted bs) as [inb [fm Hm]].
+      destruct (M.all_ballots_counted bs) as [inb [fm Hm]].
       pose proof (margin_same_from_both_existential bs ebs pbs H0 H1 _ Hm
                                                     [] inb fm eq_refl).
       destruct X as [ets [etinbs [tpbs [etpbs [em He]]]]].
@@ -1297,26 +1302,26 @@ Module Encschulze (Import C : Cand) (Import K : Keys) (Import Crp : CryptoAxioms
       assert (ets = []). destruct ets. auto.
       rewrite H in Htpb. inversion Htpb. rewrite H3 in He. 
 
-      pose proof (ecdecrypt grp ebs etinbs
+      pose proof (ecdecrypt Crp.grp ebs etinbs
                             em
                             fm
                             (fun c d => construct_zero_knowledge_decryption_proof
-                                       grp privatekey (em c d)) He).
+                                       Crp.grp privatekey (em c d)) He).
       simpl in X. 
       assert (forall c d : cand,
                  verify_zero_knowledge_decryption_proof
-                   grp (fm c d) (em c d)
-                   (construct_zero_knowledge_decryption_proof grp privatekey (em c d)) = true).
+                   Crp.grp (fm c d) (em c d)
+                   (construct_zero_knowledge_decryption_proof Crp.grp privatekey (em c d)) = true).
       intros. apply verify_honest_decryption_zkp. rewrite Hfm. auto.
       specialize (X H4). clear H4.
 
-      pose proof (fin bs fm inb (c_wins fm) (wins_loses_type_dec fm) Hm
-                      (c_wins_true_type fm) (c_wins_false_type fm)).
-      pose proof (ecfin grp ebs fm (c_wins fm) (wins_loses_type_dec fm)
-                        X (c_wins_true_type fm) (c_wins_false_type fm)).
+      pose proof (M.fin bs fm inb (M.c_wins fm) (M.wins_loses_type_dec fm) Hm
+                      (M.c_wins_true_type fm) (M.c_wins_false_type fm)).
+      pose proof (ecfin Crp.grp ebs fm (M.c_wins fm) (M.wins_loses_type_dec fm)
+                        X (M.c_wins_true_type fm) (M.c_wins_false_type fm)).
       
       (* All I need now is assert c_wins fm = w *)
-      pose proof (uniqueness_proof bs w (c_wins fm) H2 X0).
+      pose proof (uniqueness_proof bs w (M.c_wins fm) H2 X0).
       rewrite H4. assumption.
     Qed.
 
@@ -1326,14 +1331,14 @@ Module Encschulze (Import C : Cand) (Import K : Keys) (Import Crp : CryptoAxioms
        v, and w *)
     Theorem existence_of_perm :
       forall cpi zkpcpi,
-        verify_permutation_commitment grp (Datatypes.length cand_all) cpi zkpcpi = true ->
+        verify_permutation_commitment Crp.grp (Datatypes.length cand_all) cpi zkpcpi = true ->
         existsT (pi : Permutation),  forall u v w zkppermuv zkppermvw, 
-      (forall c, verify_row_permutation_ballot grp u v cpi zkppermuv c = true) ->
-      (forall c, verify_col_permutation_ballot grp v w cpi zkppermvw c = true) ->
-      forall c d, (decrypt_message grp privatekey (v c d) =
-            decrypt_message grp privatekey (u c (projT1 pi d))) /\
-           (decrypt_message grp privatekey (w c d) =
-            decrypt_message grp privatekey (v (projT1 pi c) d)).
+      (forall c, verify_row_permutation_ballot Crp.grp u v cpi zkppermuv c = true) ->
+      (forall c, verify_col_permutation_ballot Crp.grp v w cpi zkppermvw c = true) ->
+      forall c d, (decrypt_message Crp.grp privatekey (v c d) =
+            decrypt_message Crp.grp privatekey (u c (projT1 pi d))) /\
+           (decrypt_message Crp.grp privatekey (w c d) =
+            decrypt_message Crp.grp privatekey (v (projT1 pi c) d)).
     Proof.
       intros. pose proof (perm_axiom cpi zkpcpi H).  
       destruct X as [pi X]. 
@@ -1349,29 +1354,29 @@ Module Encschulze (Import C : Cand) (Import K : Keys) (Import Crp : CryptoAxioms
     
     (* Correctness in reverse direction. From encrypted ballots to plaintext *)
     Lemma margin_same_from_both_existential_rev 
-          (bs : list ballot) (ebs : list eballot) (pbs : list pballot)
-          (Ht : pbs = map (fun x => (fun c d => decrypt_message grp privatekey (x c d))) ebs)
+          (bs : list M.ballot) (ebs : list eballot) (pbs : list pballot)
+          (Ht : pbs = map (fun x => (fun c d => decrypt_message Crp.grp privatekey (x c d))) ebs)
           (H1 : mapping_ballot_pballot bs pbs) :
       forall (s : EState),
-        ECount grp ebs s ->
+        ECount Crp.grp ebs s ->
         forall (ets etinbs : list eballot)
           (tpbs etpbs : list pballot)
           (em : cand -> cand -> ciphertext)
-          (H2 : tpbs = map (fun x => (fun c d => decrypt_message grp privatekey (x c d))) ets)
-          (H3 : etpbs = map (fun x => (fun c d => decrypt_message grp privatekey (x c d))) etinbs),
+          (H2 : tpbs = map (fun x => (fun c d => decrypt_message Crp.grp privatekey (x c d))) ets)
+          (H3 : etpbs = map (fun x => (fun c d => decrypt_message Crp.grp privatekey (x c d))) etinbs),
           s = epartial (ets, etinbs) em ->
           existsT
-            (ts tinbs : list ballot)
+            (ts tinbs : list M.ballot)
             (m : cand -> cand -> Z), 
-      (Count bs (partial (ts, tinbs) m) *
-       (m = fun c d => decrypt_message grp privatekey (em c d)) *
+      (M.Count bs (M.partial (ts, tinbs) m) *
+       (m = fun c d => decrypt_message Crp.grp privatekey (em c d)) *
        mapping_ballot_pballot ts tpbs *
        mapping_ballot_pballot tinbs etpbs)%type.
     Proof.
       intros s H.
       induction H; intros. inversion H. 
       exists bs, [], decm.
-      pose proof (ax bs bs decm eq_refl e0).
+      pose proof (M.ax bs bs decm eq_refl e0).
       repeat split.  auto.
       (* Now from e1, I need to infer that decm is honest decryption of em *)
       apply functional_extensionality; intros.
@@ -1390,7 +1395,7 @@ Module Encschulze (Import C : Cand) (Import K : Keys) (Import Crp : CryptoAxioms
          I am going to add u in encrypted margin *)
       inversion H0.
       specialize (IHECount (u :: us) inbs). simpl in IHECount.
-      specialize (IHECount ((fun c d : cand => decrypt_message grp privatekey (u c d)) :: tpbs)
+      specialize (IHECount ((fun c d : cand => decrypt_message Crp.grp privatekey (u c d)) :: tpbs)
                            etpbs m).
       rewrite H2 in IHECount. rewrite H5 in IHECount.
       specialize (IHECount eq_refl).
@@ -1409,30 +1414,30 @@ Module Encschulze (Import C : Cand) (Import K : Keys) (Import Crp : CryptoAxioms
          I know b is valid so this translates back to validity of u. 
          Since u is valid then b0 is valid *)
       assert (matrix_ballot_valid
-                (fun c d : cand => decrypt_message grp privatekey (u c d))).
+                (fun c d : cand => decrypt_message Crp.grp privatekey (u c d))).
       pose proof (existence_of_perm cpi zkpcpi e). 
       destruct X as [[pi Hsig] Hf].
       specialize (Hf u v w zkppermuv zkppermvw e0 e1).
       destruct m0 as [Min [fn Mas]].
 
-     assert (forall c d, decrypt_message grp privatekey (v c d) =
-                     decrypt_message grp privatekey (u c (pi d))). 
+     assert (forall c d, decrypt_message Crp.grp privatekey (v c d) =
+                     decrypt_message Crp.grp privatekey (u c (pi d))). 
      intros. pose proof (Hf c d).
      simpl in H9. destruct H9. assumption.
 
-     assert (forall c d, decrypt_message grp privatekey (w c d) =
-                    decrypt_message grp privatekey (v (pi c) d)). 
+     assert (forall c d, decrypt_message Crp.grp privatekey (w c d) =
+                    decrypt_message Crp.grp privatekey (v (pi c) d)). 
      intros. pose proof (Hf c d). destruct H10. assumption.
 
-     assert (forall c d, decrypt_message grp privatekey (w c d) =
-                    decrypt_message grp privatekey (u (pi c) (pi d))).
+     assert (forall c d, decrypt_message Crp.grp privatekey (w c d) =
+                    decrypt_message Crp.grp privatekey (u (pi c) (pi d))).
      intros. rewrite H10. rewrite H9. auto.
 
-     assert (forall c d, b c d = decrypt_message grp privatekey (w c d)).
+     assert (forall c d, b c d = decrypt_message Crp.grp privatekey (w c d)).
      intros. pose proof (decryption_from_zkp_proof (w c d) (b c d) (zkpdecw c d) (e2 c d));
                assumption.
 
-     assert (forall c d, b c d = decrypt_message grp privatekey (u (pi c) (pi d))).
+     assert (forall c d, b c d = decrypt_message Crp.grp privatekey (u (pi c) (pi d))).
      intros.  rewrite H12. auto.
  
      split. intros. unfold Bijective in Hsig.
@@ -1450,24 +1455,25 @@ Module Encschulze (Import C : Cand) (Import K : Keys) (Import Crp : CryptoAxioms
      
      pose proof (proj2 (connect_validity_of_ballot_pballot
                            b0
-                           (fun c d : cand => decrypt_message grp privatekey (u c d)) H4)).
+                           (fun c d : cand => decrypt_message Crp.grp privatekey (u c d)) H4)).
       assert ( forall c : cand, (b0 c > 0)%nat).
-      destruct ((matrix_ballot_valid_dec (fun c d : cand => decrypt_message grp privatekey (u c d)))).
+      destruct ((matrix_ballot_valid_dec (fun c d : cand =>
+                                            decrypt_message Crp.grp privatekey (u c d)))).
       simpl in H10. specialize (H10 eq_refl).
-      destruct (ballot_valid_dec b0). auto. inversion H10. congruence.
+      destruct (M.ballot_valid_dec b0). auto. inversion H10. congruence.
       (* Add this ballot in count *)
-      pose proof (cvalid bs b0 ts decm
-                         (fun c d : cand => decrypt_message grp privatekey (nm c d))
+      pose proof (M.cvalid bs b0 ts decm
+                         (fun c d : cand => decrypt_message Crp.grp privatekey (nm c d))
                          tinbs IHc H11).
       unfold map_ballot_pballot in H4.      
       assert (
           forall c d : cand,
             ((b0 c < b0 d)%nat ->
-             (fun c0 d0 : cand => decrypt_message grp privatekey (nm c0 d0)) c d = decm c d + 1) /\
-            (b0 c = b0 d -> (fun c0 d0 : cand => decrypt_message grp privatekey (nm c0 d0)) c d
+             (fun c0 d0 : cand => decrypt_message Crp.grp privatekey (nm c0 d0)) c d = decm c d + 1) /\
+            (b0 c = b0 d -> (fun c0 d0 : cand => decrypt_message Crp.grp privatekey (nm c0 d0)) c d
                            = decm c d) /\
             ((b0 c > b0 d)%nat ->
-             (fun c0 d0 : cand => decrypt_message grp privatekey (nm c0 d0)) c d = decm c d - 1)).
+             (fun c0 d0 : cand => decrypt_message Crp.grp privatekey (nm c0 d0)) c d = decm c d - 1)).
       destruct H4.  destruct H4.  congruence.
       destruct H4. destruct H12.  
       intros.
@@ -1484,7 +1490,7 @@ Module Encschulze (Import C : Cand) (Import K : Keys) (Import Crp : CryptoAxioms
       apply H16 in H14.  rewrite e3. rewrite homomorphic_addition_axiom.
       rewrite H14.  rewrite Hdec. rewrite Z.add_comm. auto.
       specialize (X H12).
-      exists ts, tinbs, (fun c d : cand => decrypt_message grp privatekey (nm c d)).
+      exists ts, tinbs, (fun c d : cand => decrypt_message Crp.grp privatekey (nm c d)).
       split. split. split. auto. rewrite H7. auto.  rewrite <- H2 in H8. auto.
       auto.
       (* Finished cvalid case *)
@@ -1497,7 +1503,7 @@ Module Encschulze (Import C : Cand) (Import K : Keys) (Import Crp : CryptoAxioms
       inversion H6. 
       specialize (IHECount (u :: us) etinbs).
       simpl in IHECount.
-      specialize (IHECount ((fun c d : cand => decrypt_message grp privatekey (u c d)) :: tpbs)).
+      specialize (IHECount ((fun c d : cand => decrypt_message Crp.grp privatekey (u c d)) :: tpbs)).
       simpl in H3. destruct etpbs. inversion H3.
       inversion H3.
       specialize (IHECount etpbs m). rewrite <- H5 in H2.
@@ -1516,7 +1522,7 @@ Module Encschulze (Import C : Cand) (Import K : Keys) (Import Crp : CryptoAxioms
        I know b is invalid so this translates back to invalidity of u. 
          Since u is invalid then b0 is invalid *)
       assert (~matrix_ballot_valid
-               (fun c d : cand => decrypt_message grp privatekey (u c d))).
+               (fun c d : cand => decrypt_message Crp.grp privatekey (u c d))).
       intro. apply n.
       
       unfold matrix_ballot_valid in *.  destruct H14 as [H14 [g Hg]].
@@ -1525,24 +1531,24 @@ Module Encschulze (Import C : Cand) (Import K : Keys) (Import Crp : CryptoAxioms
       destruct X as [[pi Hsig] Hf].
       specialize (Hf u v w zkppermuv zkppermvw e0 e1).
       
-      assert (forall c d, decrypt_message grp privatekey (v c d) =
-                     decrypt_message grp privatekey (u c (pi d))). 
+      assert (forall c d, decrypt_message Crp.grp privatekey (v c d) =
+                     decrypt_message Crp.grp privatekey (u c (pi d))). 
       intros. pose proof (Hf c d).
       simpl in H15. destruct H15. assumption.
       
-      assert (forall c d, decrypt_message grp privatekey (w c d) =
-                     decrypt_message grp privatekey (v (pi c) d)). 
+      assert (forall c d, decrypt_message Crp.grp privatekey (w c d) =
+                     decrypt_message Crp.grp privatekey (v (pi c) d)). 
       intros. pose proof (Hf c d). simpl in H16. destruct H16. assumption.
       
-      assert (forall c d, decrypt_message grp privatekey (w c d) =
-                     decrypt_message grp privatekey (u (pi c) (pi d))).
+      assert (forall c d, decrypt_message Crp.grp privatekey (w c d) =
+                     decrypt_message Crp.grp privatekey (u (pi c) (pi d))).
       intros. rewrite H16. rewrite H15. auto.
       
-      assert (forall c d, b c d = decrypt_message grp privatekey (w c d)).
+      assert (forall c d, b c d = decrypt_message Crp.grp privatekey (w c d)).
       intros. pose proof (decryption_from_zkp_proof (w c d) (b c d) (zkpdecw c d) (e2 c d));
                 assumption.
       
-      assert (forall c d, b c d = decrypt_message grp privatekey (u (pi c) (pi d))).
+      assert (forall c d, b c d = decrypt_message Crp.grp privatekey (u (pi c) (pi d))).
       intros.  rewrite H18. auto.
       
       
@@ -1556,12 +1562,12 @@ Module Encschulze (Import C : Cand) (Import K : Keys) (Import Crp : CryptoAxioms
       
       pose proof (proj2 (connect_invalidity_of_ballot_pballot
                            b0
-                           (fun c d : cand => decrypt_message grp privatekey (u c d)) H8)).
+                           (fun c d : cand => decrypt_message Crp.grp privatekey (u c d)) H8)).
       assert (exists c, (b0 c = 0)%nat). 
-      destruct (matrix_ballot_valid_dec (fun c d : cand => decrypt_message grp privatekey (u c d))).
+      destruct (matrix_ballot_valid_dec (fun c d : cand => decrypt_message Crp.grp privatekey (u c d))).
       congruence. simpl in H15. specialize (H15 eq_refl).
-      destruct (ballot_valid_dec b0). inversion H15.  auto.
-      pose proof (cinvalid bs b0 ts decm tinbs IHc H16).
+      destruct (M.ballot_valid_dec b0). inversion H15.  auto.
+      pose proof (M.cinvalid bs b0 ts decm tinbs IHc H16).
       exists ts, (b0 :: tinbs), decm.
       split. split. split. auto.
       rewrite H7 in Hdec. auto.
@@ -1580,10 +1586,10 @@ Module Encschulze (Import C : Cand) (Import K : Keys) (Import Crp : CryptoAxioms
     (* This function computes the encrypted margin *)
     Fixpoint compute_margin_enc (bs : list eballot) :=
       match bs with
-      | [] => fun c d => encrypt_message grp 0
+      | [] => fun c d => encrypt_message Crp.grp 0
       | h :: t =>
-        match matrix_ballot_valid_dec (fun c d => decrypt_message grp privatekey (h c d)) with
-        | left _ => fun c d => homomorphic_addition grp (h c d) (compute_margin_enc t c d)
+        match matrix_ballot_valid_dec (fun c d => decrypt_message Crp.grp privatekey (h c d)) with
+        | left _ => fun c d => homomorphic_addition Crp.grp (h c d) (compute_margin_enc t c d)
         | right _ => compute_margin_enc t
         end
       end.
@@ -1593,18 +1599,20 @@ Module Encschulze (Import C : Cand) (Import K : Keys) (Import Crp : CryptoAxioms
       
     Lemma valid_compute_margin_distributes_enc :
       forall bs (u : eballot),
-        matrix_ballot_valid (fun c d : cand => decrypt_message grp privatekey (u c d)) ->
-        forall c d, decrypt_message grp privatekey
+        matrix_ballot_valid (fun c d : cand => decrypt_message Crp.grp privatekey (u c d)) ->
+        forall c d, decrypt_message Crp.grp privatekey
                                (compute_margin_enc (bs ++ [u]) c d) =
-               decrypt_message grp privatekey
-                               (homomorphic_addition grp (u c d) (compute_margin_enc bs c d)).
+               decrypt_message Crp.grp privatekey
+                               (homomorphic_addition Crp.grp (u c d) (compute_margin_enc bs c d)).
     Proof.
       induction bs.
       + simpl; intros. 
-        destruct (matrix_ballot_valid_dec (fun c d : cand => decrypt_message grp privatekey (u c d)));
+        destruct (matrix_ballot_valid_dec (fun c d : cand =>
+                                             decrypt_message Crp.grp privatekey (u c d)));
           try congruence.
       + intros. simpl.
-        destruct (matrix_ballot_valid_dec (fun c d : cand => decrypt_message grp privatekey (a c d))).
+        destruct (matrix_ballot_valid_dec (fun c d : cand =>
+                                             decrypt_message Crp.grp privatekey (a c d))).
         pose proof (IHbs _ H).
         repeat rewrite homomorphic_addition_axiom. rewrite H0.
         rewrite homomorphic_addition_axiom. lia. auto. 
@@ -1615,10 +1623,10 @@ Module Encschulze (Import C : Cand) (Import K : Keys) (Import Crp : CryptoAxioms
 
     Lemma invalid_compute_margin_same_enc :
       forall bs (u : eballot),
-        ~matrix_ballot_valid (fun c d : cand => decrypt_message grp privatekey (u c d)) ->
-        forall c d, decrypt_message grp privatekey 
+        ~matrix_ballot_valid (fun c d : cand => decrypt_message Crp.grp privatekey (u c d)) ->
+        forall c d, decrypt_message Crp.grp privatekey 
                                (compute_margin_enc (bs ++ [u]) c d) = 
-               decrypt_message grp privatekey (compute_margin_enc bs c d).
+               decrypt_message Crp.grp privatekey (compute_margin_enc bs c d).
     Proof.
       induction bs; simpl; intros; try auto.
       destruct (matrix_ballot_valid_dec _).
@@ -1634,12 +1642,12 @@ Module Encschulze (Import C : Cand) (Import K : Keys) (Import Crp : CryptoAxioms
       
       
     Lemma tail_count_enc : forall bs s,
-        ECount grp bs s ->
+        ECount Crp.grp bs s ->
         forall us inbs m,
           s = epartial (us, inbs) m ->
           exists cs', bs = cs' ++ us /\
-                 (forall c d, decrypt_message grp privatekey (m c d) =
-                         decrypt_message grp privatekey (compute_margin_enc cs' c d)).
+                 (forall c d, decrypt_message Crp.grp privatekey (m c d) =
+                         decrypt_message Crp.grp privatekey (compute_margin_enc cs' c d)).
     Proof.
       intros bs s Hc.
       induction Hc; simpl; intros; inversion H; subst; clear H.
@@ -1657,30 +1665,30 @@ Module Encschulze (Import C : Cand) (Import K : Keys) (Import Crp : CryptoAxioms
       intros. 
       (*  m0 : matrix_ballot_valid b it means matrix_ballot_valid u 
           so add it to the counting *)
-      assert (matrix_ballot_valid (fun c d : cand => decrypt_message grp privatekey (u c d))). 
+      assert (matrix_ballot_valid (fun c d : cand => decrypt_message Crp.grp privatekey (u c d))). 
       pose proof (existence_of_perm cpi zkpcpi e). 
       destruct X as [[pi Hsig] Hf].
       specialize (Hf u v w zkppermuv zkppermvw e0 e1).
       destruct m0 as [Min [fn Mas]].
 
-      assert (forall c d, decrypt_message grp privatekey (v c d) =
-                     decrypt_message grp privatekey (u c (pi d))). 
+      assert (forall c d, decrypt_message Crp.grp privatekey (v c d) =
+                     decrypt_message Crp.grp privatekey (u c (pi d))). 
       intros. pose proof (Hf c0 d0). destruct H.
       simpl in H.  assumption.
       
-      assert (forall c d, decrypt_message grp privatekey (w c d) =
-                     decrypt_message grp privatekey (v (pi c) d)). 
+      assert (forall c d, decrypt_message Crp.grp privatekey (w c d) =
+                     decrypt_message Crp.grp privatekey (v (pi c) d)). 
       intros. pose proof (Hf c0 d0). destruct H0. assumption.
       
-      assert (forall c d, decrypt_message grp privatekey (w c d) =
-                     decrypt_message grp privatekey (u (pi c) (pi d))).
+      assert (forall c d, decrypt_message Crp.grp privatekey (w c d) =
+                     decrypt_message Crp.grp privatekey (u (pi c) (pi d))).
       intros. rewrite H0. rewrite H. auto.
       
-      assert (forall c d, b c d = decrypt_message grp privatekey (w c d)).
+      assert (forall c d, b c d = decrypt_message Crp.grp privatekey (w c d)).
       intros. pose proof (decryption_from_zkp_proof (w c0 d0) (b c0 d0)
                                                     (zkpdecw c0 d0) (e2 c0 d0)); assumption.
 
-      assert (forall c d, b c d = decrypt_message grp privatekey (u (pi c) (pi d))).
+      assert (forall c d, b c d = decrypt_message Crp.grp privatekey (u (pi c) (pi d))).
       intros. rewrite <- H3. auto.
 
       split. intros. unfold Bijective in Hsig.
@@ -1703,7 +1711,7 @@ Module Encschulze (Import C : Cand) (Import K : Keys) (Import Crp : CryptoAxioms
       (* Hypothesis n states that b is not valid so it translates 
          back to decryption of u *)
       assert (Hm :
-                ~matrix_ballot_valid (fun c d : cand => decrypt_message grp privatekey (u c d))).
+                ~matrix_ballot_valid (fun c d : cand => decrypt_message Crp.grp privatekey (u c d))).
 
 
       intro. apply n.
@@ -1714,24 +1722,24 @@ Module Encschulze (Import C : Cand) (Import K : Keys) (Import Crp : CryptoAxioms
       destruct X as [[pi Hsig] Hf].
       specialize (Hf u v w zkppermuv zkppermvw e0 e1).
 
-      assert (forall c d, decrypt_message grp privatekey (v c d) =
-                     decrypt_message grp privatekey (u c (pi d))). 
+      assert (forall c d, decrypt_message Crp.grp privatekey (v c d) =
+                     decrypt_message Crp.grp privatekey (u c (pi d))). 
       intros. pose proof (Hf c d).
       simpl in H0. destruct H0. assumption.
 
-      assert (forall c d, decrypt_message grp privatekey (w c d) =
-                     decrypt_message grp privatekey (v (pi c) d)). 
+      assert (forall c d, decrypt_message Crp.grp privatekey (w c d) =
+                     decrypt_message Crp.grp privatekey (v (pi c) d)). 
       intros. pose proof (Hf c d). simpl in H1. destruct H1. assumption.
 
-      assert (forall c d, decrypt_message grp privatekey (w c d) =
-                     decrypt_message grp privatekey (u (pi c) (pi d))).
+      assert (forall c d, decrypt_message Crp.grp privatekey (w c d) =
+                     decrypt_message Crp.grp privatekey (u (pi c) (pi d))).
       intros. rewrite H1. rewrite H0. auto.
 
-      assert (forall c d, b c d = decrypt_message grp privatekey (w c d)).
+      assert (forall c d, b c d = decrypt_message Crp.grp privatekey (w c d)).
       intros. pose proof (decryption_from_zkp_proof (w c d) (b c d) (zkpdecw c d) (e2 c d));
                 assumption.
 
-      assert (forall c d, b c d = decrypt_message grp privatekey (u (pi c) (pi d))).
+      assert (forall c d, b c d = decrypt_message Crp.grp privatekey (u (pi c) (pi d))).
       intros. rewrite H3. auto.
 
       split. intros. unfold Bijective in Hsig.
@@ -1753,11 +1761,11 @@ Module Encschulze (Import C : Cand) (Import K : Keys) (Import Crp : CryptoAxioms
     
 
     Lemma same_margin_enc :
-      forall bs inbs inbs0 encm encm0 s s0 (c0 : ECount grp bs s) (c1 :  ECount grp bs s0),  
+      forall bs inbs inbs0 encm encm0 s s0 (c0 : ECount Crp.grp bs s) (c1 :  ECount Crp.grp bs s0),  
         s = epartial ([], inbs) encm ->
         s0 = epartial ([], inbs0) encm0 ->
-        forall c d, decrypt_message grp privatekey (encm c d) =
-               decrypt_message grp privatekey (encm0 c d). 
+        forall c d, decrypt_message Crp.grp privatekey (encm c d) =
+               decrypt_message Crp.grp privatekey (encm0 c d). 
     Proof.
       intros.
       pose proof (tail_count_enc bs s c0 [] inbs encm H).
@@ -1771,7 +1779,7 @@ Module Encschulze (Import C : Cand) (Import K : Keys) (Import Crp : CryptoAxioms
       
     
     Lemma unique_dec_margin : forall bs dm dm0,
-      ECount grp bs (edecrypt dm) ->  ECount grp bs (edecrypt dm0) ->
+      ECount Crp.grp bs (edecrypt dm) ->  ECount Crp.grp bs (edecrypt dm0) ->
       dm = dm0.
     Proof.
       intros. inversion X. inversion X0. subst.
@@ -1794,7 +1802,7 @@ Module Encschulze (Import C : Cand) (Import K : Keys) (Import Crp : CryptoAxioms
       
     
     Lemma uniqueness_proof_enc : forall bs w w',
-        ECount grp bs (ewinners w) -> ECount grp bs (ewinners w') -> w = w'.
+        ECount Crp.grp bs (ewinners w) -> ECount Crp.grp bs (ewinners w') -> w = w'.
     Proof. 
       intros bs w w' H1 H2.
       inversion H1. inversion  H2. 
@@ -1810,32 +1818,32 @@ Module Encschulze (Import C : Cand) (Import K : Keys) (Import Crp : CryptoAxioms
       specialize ((proj1 H0) eq_refl); intros.
       destruct H. destruct H4.
       destruct H3. destruct H5.
-      pose proof (loses_type_prop dm0 x x0).
-      pose proof (loses_prop_iterated_marg dm0 x H9).
+      pose proof (M.loses_type_prop dm0 x x0).
+      pose proof (M.loses_prop_iterated_marg dm0 x H9).
       destruct H10 as [dd H10].
-      pose proof (wins_type_prop dm0 x x1).
-      pose proof (wins_prop_iterated_marg dm0 x H11).
+      pose proof (M.wins_type_prop dm0 x x1).
+      pose proof (M.wins_prop_iterated_marg dm0 x H11).
       pose proof (H12 dd). omega.
 
       specialize ((proj1 H3) eq_refl); intros.
       specialize ((proj1 H5) eq_refl); intros.
       destruct H. destruct H4.
       destruct H3. destruct H5.
-      pose proof (loses_type_prop dm0 x x0).
-      pose proof (loses_prop_iterated_marg dm0 x H9).
+      pose proof (M.loses_type_prop dm0 x x0).
+      pose proof (M.loses_prop_iterated_marg dm0 x H9).
       destruct H10 as [dd H10].
-      pose proof (wins_type_prop dm0 x x1).
-      pose proof (wins_prop_iterated_marg dm0 x H11).
+      pose proof (M.wins_type_prop dm0 x x1).
+      pose proof (M.wins_prop_iterated_marg dm0 x H11).
       pose proof (H12 dd). omega.
     Qed.
       
  
     Lemma homomorphic_schulze_to_plaintext:
-      forall  (bs : list ballot) (pbs : list pballot) (ebs : list eballot)
+      forall  (bs : list M.ballot) (pbs : list pballot) (ebs : list eballot)
          (w : cand -> bool)
-         (H : pbs = map (fun x => (fun c d => decrypt_message grp privatekey (x c d))) ebs)
+         (H : pbs = map (fun x => (fun c d => decrypt_message Crp.grp privatekey (x c d))) ebs)
          (H2 : mapping_ballot_pballot bs pbs), (* valid b <-> valid pb *)
-        ECount grp ebs (ewinners w) -> Count bs (winners w).
+        ECount Crp.grp ebs (ewinners w) -> M.Count bs (M.winners w).
     Proof.
       intros bs pbs ebs w H0 H1 H2.
       destruct (pall_ballots_counted ebs) as [inb [fm Hm]]. 
@@ -1843,30 +1851,31 @@ Module Encschulze (Import C : Cand) (Import K : Keys) (Import Crp : CryptoAxioms
                      bs ebs pbs H0 H1 _ Hm [] inb []
                     (map
                        (fun (x : cand -> cand -> ciphertext)
-                          (c d : cand) => decrypt_message grp privatekey (x c d)) inb)
+                          (c d : cand) => decrypt_message Crp.grp privatekey (x c d)) inb)
                  fm eq_refl eq_refl eq_refl).
       destruct X as [ts [tinbs [m [[[IHc Hmm] IHm] Hw]]]].    
       assert (ts = []). destruct ts. reflexivity. inversion IHm.
       rewrite H in IHc, IHm.
-      pose proof (ecdecrypt grp ebs inb fm m
+      pose proof (ecdecrypt Crp.grp ebs inb fm m
                  (fun c d => construct_zero_knowledge_decryption_proof
-                            grp privatekey (fm c d)) Hm).
+                            Crp.grp privatekey (fm c d)) Hm).
       simpl in X.
       assert (forall c d : cand,
                  verify_zero_knowledge_decryption_proof
-                   grp (m c d) (fm c d)
-                   (construct_zero_knowledge_decryption_proof grp privatekey (fm c d)) = true).
+                   Crp.grp (m c d) (fm c d)
+                   (construct_zero_knowledge_decryption_proof Crp.grp privatekey (fm c d)) = true).
       intros. apply verify_honest_decryption_zkp. rewrite Hmm. auto.
       specialize (X H3). clear H3. 
-      pose proof (fin bs m tinbs (c_wins m) (wins_loses_type_dec m) IHc
-                      (c_wins_true_type m) (c_wins_false_type m)).
-      pose proof (ecfin grp ebs m (c_wins m) (wins_loses_type_dec m)
-                        X (c_wins_true_type m) (c_wins_false_type m)).
+      pose proof (M.fin bs m tinbs (M.c_wins m) (M.wins_loses_type_dec m) IHc
+                      (M.c_wins_true_type m) (M.c_wins_false_type m)).
+      pose proof (ecfin Crp.grp ebs m (M.c_wins m) (M.wins_loses_type_dec m)
+                        X (M.c_wins_true_type m) (M.c_wins_false_type m)).
       (* I need uniqueness proof stating that 
          ECount grp ebs (ewinners w) ->  ECount grp ebs (ewinners (c_wins m)) -> 
          w = c_wins m *)  
       pose proof (uniqueness_proof_enc ebs _ _ H2 X1).
       rewrite H3. auto. 
     Qed.
-                                                                        
+
+End Encschulze.
 
